chapter02-spec/solutions/exercise02_solution.dfy
@@ -1,44 +1,44 @@
-//#title IsPrime
+//#title IsPrime II
 //#desc Working with an implementation proof
 
-predicate divides(f:nat, i:nat)
-  requires 1<=f
+predicate divides(factor:nat, candidate:nat)
+  requires 1<=factor
 {
-  i % f == 0
+  candidate % factor == 0
 }
 
-predicate IsPrime(i:nat)
+predicate IsPrime(candidate:nat)
 {
-  && 1<i
-  && ( forall f :: 1 < f < i ==> !divides(f, i) )
+  && 1<candidate
+  && ( forall factor :: 1 < factor < candidate ==> !divides(factor, candidate) )
 }
 
 // Convincing the proof to go through requires adding
 // a loop invariant and a triggering assert.
-method test_prime(i:nat) returns (result:bool)
-  requires 1<i
-  ensures result == IsPrime(i)
+method test_prime(candidate:nat) returns (result:bool)
+  requires 1<candidate
+  ensures result == IsPrime(candidate)
 {
 //#exercise  // Fill in the body.
 //#start-elide
-  var f := 2;
-  while (f < i)
+  var factor := 2;
+  while (factor < candidate)
     // This loop invariant completes an inductive proof of the
     // body of IsPrime. Go look at the IsPrime definition and
     // see how this forall relates to it.
-    // Note that when f == i, this is IsPrime.
-    // Also note that, when the while loop exists, i<=f.
-    invariant forall g :: 1 < g < f ==> !divides(g, i)
+    // Note that when factor == candidate, this is IsPrime.
+    // Also note that, when the while loop exists, candidate<=factor.
+    invariant forall smallerfactor :: 1 < smallerfactor < factor ==> !divides(smallerfactor, candidate)
   {
-    if i % f == 0 {
+    if candidate % factor == 0 {
       // This assert is needed to witness that !IsPrime.
       // !IsPrime is !forall !divides, which rewrites to exists divides.
       // Dafny rarely triggers its way to a guess for an exists (apparently
       // it's tough for Z3), but mention a witness and Z3's happy.
-      assert divides(f, i);
+      assert divides(factor, candidate);
       return false;
     }
-    f := f + 1;
+    factor := factor + 1;
   }
   return true;
 //#end-elide
@@ -46,11 +46,11 @@ method test_prime(i:nat) returns (result:bool)
 
 method Main()
 {
-  var a := test_prime(3);
-  assert a;
-  var b := test_prime(4);
+  var isprime3 := test_prime(3);
+  assert isprime3;
+  var isprime4 := test_prime(4);
   assert divides(2, 4);
-  assert !b;
-  var c := test_prime(5);
-  assert c;
+  assert !isprime4;
+  var isprime5 := test_prime(5);
+  assert isprime5;
 }
