chapter01-basics/solutions/exercise23_solution.dfy
@@ -11,22 +11,22 @@ include "exercise22_solution.dfy"
 // that one, too). If in doubt about your solution to exercise22, contact 
 // an instructor during office hours to make sure you're on the right path. 
 
-method FindInBinaryTree(t:Tree, needle:int) returns (b:bool)
-    requires IsSortedTree(t)
-    ensures b <==> needle in TreeAsSequence(t)
+method FindInBinaryTree(tree:Tree, needle:int) returns (issorted:bool)
+    requires IsSortedTree(tree)
+    ensures issorted <==> needle in TreeAsSequence(tree)
 {
 //#exercise    return true;
 //#start-elide
-    if (t.Nil?) {
+    if (tree.Nil?) {
         return false;
     } else {
-        if (needle == t.value) {
+        if (needle == tree.value) {
             return true;
-        } else if (needle < t.value) {
-            var leftRet := FindInBinaryTree(t.left, needle);
+        } else if (needle < tree.value) {
+            var leftRet := FindInBinaryTree(tree.left, needle);
             return leftRet;
         } else {
-            var rightRet := FindInBinaryTree(t.right, needle);
+            var rightRet := FindInBinaryTree(tree.right, needle);
             return rightRet;
         }
     }
